Dif.lean
@@ -1,3 +1,4 @@
 import Dif.Heap
+import Dif.Hprop
 
 /- A formalization of dynamic implicit frames. -/
