Dif/Hprop.lean
@@ -2,6 +2,7 @@ import Dif.Heap
 
 namespace Dif
 
+/-- A DIF proposition. -/
 def Hprop : Type := Heap -> PermMap -> Prop
 
 end Dif
